fstar/MLS.TreeCommon.fst
@@ -35,7 +35,8 @@ let tree_remove #leaf_t #node_t #l #i t li =
 val is_tree_empty: #leaf_t:Type -> #node_t:Type -> #l:nat -> #i:tree_index l -> tree (option leaf_t) (option node_t) l i -> bool
 let rec is_tree_empty #leaf_t #node_t #l #i t =
   match t with
-  | TNode _ left right ->
+  | TNode (Some _) left right -> false
+  | TNode None left right ->
     is_tree_empty left && is_tree_empty right
   | TLeaf (Some _) -> false
   | TLeaf None -> true
@@ -50,7 +51,7 @@ let canonicalize_tree #leaf_t #node_t #l t0 =
 
 // Helper functions to add leaf / extend the tree
 
-val find_empty_leaf: #leaf_t:Type -> #node_t:Type -> #l:nat -> #i:tree_index l -> tree (option leaf_t) (option node_t) l i -> option (leaf_index l i)
+val find_empty_leaf: #leaf_t:Type -> #node_t:Type -> #l:nat -> #i:tree_index l -> t:tree (option leaf_t) (option node_t) l i -> option (li:leaf_index l i{leaf_at t li == None})
 let rec find_empty_leaf #leaf_t #node_t #l #i t =
   match t with
   | TLeaf (Some _) -> None
