fstar/MLS.TreeSync.API.Types.fst
@@ -1,16 +1,17 @@
 module MLS.TreeSync.API.Types
 
 open Comparse
+open MLS.Crypto
 open MLS.NetworkTypes
 open MLS.TreeSync.NetworkTypes
-open MLS.TreeSync.Level1.Types
+open MLS.TreeSync.Level2.Types
 
 (** TreeSync state and accessors *)
-type treesync_state (bytes:Type0) {|bytes_like bytes|} (tkt:treekem_types bytes) = {
+type treesync_state (bytes:Type0) {|crypto_bytes bytes|} (tkt:treekem_types bytes) = {
   group_id: mls_bytes bytes;
   levels: nat;
   tree: treesync bytes tkt levels 0;
   version: nat;
 }
 
-type treesync_index (#bytes:Type0) {|bytes_like bytes|} (#tkt:treekem_types bytes) (st:treesync_state bytes tkt) = i:nat{i < pow2 st.levels}
+type treesync_index (#bytes:Type0) {|crypto_bytes bytes|} (#tkt:treekem_types bytes) (st:treesync_state bytes tkt) = i:nat{i < pow2 st.levels}
