fstar/MLS.MiscLemmas.fst
@@ -1,0 +1,15 @@
+module MLS.MiscLemmas
+
+val list_for_all_eq: #a:eqtype -> p:(a -> bool) -> l:list a -> Lemma
+  (List.Tot.for_all p l <==> (forall x. List.Tot.mem x l ==> p x))
+let rec list_for_all_eq #a p l =
+  match l with
+  | [] -> ()
+  | h::t -> list_for_all_eq p t
+
+val mem_filter: #a:eqtype -> p:(a -> bool) -> l:list a -> x:a -> Lemma
+  (List.Tot.mem x (List.Tot.filter p l) <==> (p x /\ List.Tot.mem x l))
+let rec mem_filter #a p l x =
+  match l with
+  | [] -> ()
+  | h::t -> mem_filter p t x
