fstar/MLS.TreeCommon.Lemmas.fst
@@ -1,0 +1,18 @@
+module MLS.TreeCommon.Lemmas
+
+open MLS.TreeCommon
+
+#set-options "--fuel 0 --ifuel 0"
+
+#push-options "--ifuel 2 --fuel 2"
+val mem_insert_sorted: #a:eqtype{a `subtype_of` int} -> x:a -> l:list a -> elem:a -> Lemma
+  (List.Tot.mem elem (insert_sorted x l) <==> elem == x \/ List.Tot.mem elem l)
+let rec mem_insert_sorted x l elem =
+  match l with
+  | [] -> ()
+  | [y] -> ()
+  | y::z::t ->
+    if x < y then ()
+    else if x = y then ()
+    else mem_insert_sorted x (z::t) elem
+#pop-options
