fstar/MLS.TreeSync.Level1.Proofs.fst
@@ -1,0 +1,888 @@
+module MLS.TreeSync.Level1.Proofs
+
+open Comparse
+open MLS.Crypto
+open MLS.NetworkTypes
+open MLS.TreeSync.NetworkTypes
+open MLS.Tree
+open MLS.TreeCommon
+open MLS.TreeCommon.Lemmas
+open MLS.Tree.Lemmas
+open MLS.TreeSync.ParentHash
+open MLS.TreeSync.Level0
+open MLS.TreeSync.Level0.Invariants
+open MLS.TreeSync.Level1.Types
+open MLS.TreeSync.Level1
+open MLS.TreeSync.Level1.Invariants
+open MLS.MiscLemmas
+
+#set-options "--fuel 1 --ifuel 1"
+
+(*** Utility functions ***)
+
+val node_index_inside_tree: #leaf_t:Type -> #node_t:Type -> #l:nat -> #i:tree_index l -> node_index -> tree leaf_t node_t l i -> bool
+let node_index_inside_tree #leaf_t #node_t #l #i (|xl, xi|) _ =
+  xl <= l && leaf_index_inside l i xi
+
+(*** Misc lemmas ***)
+
+val mem_ul_eq: x:nat -> l:list (nat_lbytes 4) -> Lemma
+  (mem_ul x l <==> x < pow2 32 /\ (List.Tot.mem x l))
+let rec mem_ul_eq x l =
+  match l with
+  | [] -> ()
+  | h::t -> mem_ul_eq x t
+
+val mem_ul_insert_sorted: x:nat_lbytes 4 -> l:list (nat_lbytes 4) -> elem:nat -> Lemma
+  (mem_ul elem (insert_sorted x l) <==> elem == x \/ mem_ul elem l)
+let mem_ul_insert_sorted x l elem =
+  mem_ul_eq elem (insert_sorted x l);
+  mem_ul_eq elem l;
+  if elem < pow2 32 then mem_insert_sorted x l elem
+  else ()
+
+val mem_ul_filter: p:(nat -> bool) -> l:list (nat_lbytes 4) -> x:nat -> Lemma
+  (mem_ul x (List.Tot.filter p l) <==> (p x /\ mem_ul x l))
+let rec mem_ul_filter p l x =
+  match l with
+  | [] -> ()
+  | h::t -> mem_ul_filter p t x
+
+val mem_unmerged_resolution_eq: l:list (nat_lbytes 4) -> x:node_index -> Lemma
+  (List.Tot.mem x (unmerged_resolution l) <==> (let (|xl, xi|) = x in xl == 0 /\ mem_ul xi l))
+let rec mem_unmerged_resolution_eq l x =
+  match l with
+  | [] -> ()
+  | h::t -> mem_unmerged_resolution_eq t x
+
+(*** set_eqP ***)
+
+val set_eqP: #a:eqtype -> list a -> list a -> prop
+let set_eqP #a l1 l2 =
+  forall x. (List.Tot.mem x l1) <==> (List.Tot.mem x l2)
+
+val set_eq_to_set_eqP: #a:eqtype -> l1:list a -> l2:list a -> Lemma
+  (requires set_eq l1 l2) (ensures set_eqP l1 l2)
+let set_eq_to_set_eqP #a l1 l2 =
+  list_for_all_eq (set_equal_mem l1) l2;
+  list_for_all_eq (set_equal_mem l2) l1
+
+val set_eqP_to_set_eq: #a:eqtype -> l1:list a -> l2:list a -> Lemma
+  (requires set_eqP l1 l2) (ensures set_eq l1 l2)
+let set_eqP_to_set_eq #a l1 l2 =
+  list_for_all_eq (set_equal_mem l1) l2;
+  list_for_all_eq (set_equal_mem l2) l1
+
+(*** resolution lemmas ***)
+
+val list_for_all_eq_ul: p:(nat -> bool) -> l:list (nat_lbytes 4) -> Lemma
+  (List.Tot.for_all p l <==> (forall x. mem_ul x l ==> p x))
+let rec list_for_all_eq_ul p l =
+  match l with
+  | [] -> ()
+  | h::t -> list_for_all_eq_ul p t
+
+#push-options "--fuel 2 --ifuel 2"
+val resolution_inside_tree: #bytes:Type0 -> {|bytes_like bytes|} -> #tkt:treekem_types bytes -> #l:nat -> #i:tree_index l -> t:treesync bytes tkt l i -> x:node_index -> Lemma
+  (requires List.Tot.mem x (resolution t))
+  (ensures node_index_inside_tree x t)
+let rec resolution_inside_tree #bytes #bl #tkt #l #i t x =
+  match t with
+  | TLeaf _ -> ()
+  | TNode None left right -> (
+    List.Tot.append_mem (resolution left) (resolution right) x;
+    if List.Tot.mem x (resolution left) then
+      resolution_inside_tree left x
+    else
+      resolution_inside_tree right x
+  )
+  | TNode (Some content) _ _ -> (
+    if x = (|l, i|) then ()
+    else (
+      mem_unmerged_resolution_eq content.unmerged_leaves x;
+      list_for_all_eq_ul (unmerged_leaf_exists t) content.unmerged_leaves
+    )
+  )
+#pop-options
+
+val blank_leaf_not_in_resolution: #bytes:Type0 -> {|bytes_like bytes|} -> #tkt:treekem_types bytes -> #l:nat -> #i:tree_index l -> t:treesync bytes tkt l i -> li:leaf_index l i{leaf_at t li == None} -> Lemma
+  (not (List.Tot.mem (|0, li|) (resolution t)))
+let rec blank_leaf_not_in_resolution #bytes #bl #tkt #l #i t li =
+  match t with
+  | TLeaf _ -> ()
+  | TNode None left right -> (
+    List.Tot.append_mem (resolution left) (resolution right) (|0, li|);
+    if List.Tot.mem (|0, li|) (resolution t) then (
+      match is_left_leaf li, List.Tot.mem (|0, li|) (resolution left) with
+      | true, true -> (
+        blank_leaf_not_in_resolution left li;
+        assert(False)
+      )
+      | false, false -> (
+        blank_leaf_not_in_resolution right li;
+        assert(False)
+      )
+      | true, false -> (
+        resolution_inside_tree right (|0, li|);
+        assert(False)
+      )
+      | false, true -> (
+        resolution_inside_tree left (|0, li|);
+        assert(False)
+      )
+    ) else ()
+  )
+  | TNode (Some content) _ _ -> (
+    list_for_all_eq_ul (unmerged_leaf_exists t) content.unmerged_leaves;
+    mem_unmerged_resolution_eq content.unmerged_leaves (|0, li|)
+  )
+
+(*** last_update eq lemmas ***)
+
+val mem_last_update_lhs_eq: #bytes:Type0 -> {|bytes_like bytes|} -> #tkt:treekem_types bytes -> #lu:nat -> #lp:nat{lu < lp} -> #iu:tree_index lu -> #ip:tree_index lp{leaf_index_inside lp ip iu} -> u:treesync bytes tkt lu iu -> p:treesync bytes tkt lp ip{node_not_blank p} -> x:node_index -> Lemma
+  (List.Tot.mem x (last_update_lhs u p) <==> (
+    let (c, _) = get_child_sibling p iu in
+    (List.Tot.mem x (resolution c) /\ x <> (|lu, iu|))
+  ))
+let mem_last_update_lhs_eq #bytes #bl #tkt #lu #lp #iu #ip u p x =
+  let (c, _) = get_child_sibling p iu in
+  mem_filter (op_disEquality (|lu, iu|)) (resolution c) x
+
+val mem_last_update_rhs_eq: #bytes:Type0 -> {|bytes_like bytes|} -> #tkt:treekem_types bytes -> #lu:nat -> #lp:nat{lu < lp} -> #iu:tree_index lu -> #ip:tree_index lp{leaf_index_inside lp ip iu} -> u:treesync bytes tkt lu iu -> p:treesync bytes tkt lp ip{node_not_blank p} -> x:node_index -> Lemma
+  (List.Tot.mem x (last_update_rhs u p) <==> (
+    let (c, _) = get_child_sibling p iu in
+    let p_unmerged_leaves = (Some?.v (TNode?.data p)).unmerged_leaves in
+    let (|xl, xi|) = x in
+    (xl == 0 /\ leaf_index_inside_tree c xi /\ mem_ul xi p_unmerged_leaves)
+  ))
+let mem_last_update_rhs_eq #bytes #bl #tkt #lu #lp #iu #ip u p x =
+  let (c, _) = get_child_sibling p iu in
+  let p_unmerged_leaves = (Some?.v (TNode?.data p)).unmerged_leaves in
+  let (|xl, xi|) = x in
+  mem_unmerged_resolution_eq (List.Tot.filter (leaf_index_inside_tree c) p_unmerged_leaves) x;
+  mem_ul_filter (leaf_index_inside_tree c) p_unmerged_leaves xi
+
+(*** prop invariant definition ***)
+
+val is_subtree_of: #bytes:Type0 -> {|bytes_like bytes|} -> #tkt:treekem_types bytes -> #lu:nat -> #lp:nat{lu <= lp} -> #iu:tree_index lu -> #ip:tree_index lp{leaf_index_inside lp ip iu} -> treesync bytes tkt lu iu -> treesync bytes tkt lp ip -> prop
+let rec is_subtree_of #bytes #bl #tkt #lu #lp #iu #ip u p =
+  if lu = lp then (
+    iu == ip /\ u == p
+  ) else (
+    let (p_child, _) = get_child_sibling p iu in
+    is_subtree_of u p_child
+  )
+
+val parent_hash_linkedP: #bytes:Type0 -> {|crypto_bytes bytes|} -> #tkt:treekem_types bytes -> #lu:nat -> #lp:nat{lu < lp} -> #iu:tree_index lu -> #ip:tree_index lp{leaf_index_inside lp ip iu} -> u:treesync bytes tkt lu iu{node_has_parent_hash u} -> p:treesync bytes tkt lp ip{node_not_blank p} -> prop
+let parent_hash_linkedP #bytes #cb #tkt #lu #lp #iu #ip u p =
+  is_subtree_of u p /\ parent_hash_linked u p
+
+val node_has_parent_hash_linkP: #bytes:Type0 -> {|crypto_bytes bytes|} -> #tkt:treekem_types bytes -> #lp:nat -> #ip:tree_index lp -> treesync bytes tkt lp ip -> prop
+let node_has_parent_hash_linkP #bytes #cb #tkt #lp #ip p =
+  (TNode? p /\ node_not_blank p) ==> (
+    exists (lu:nat) (iu:tree_index lu) (u:treesync bytes tkt lu iu). (
+      lu < lp /\
+      leaf_index_inside lp ip iu /\
+      node_has_parent_hash u /\
+      parent_hash_linkedP u p
+    )
+  )
+
+val parent_hash_invariantP: #bytes:Type0 -> {|crypto_bytes bytes|} -> #tkt:treekem_types bytes -> #lp:nat -> #ip:tree_index lp -> t:treesync bytes tkt lp ip -> prop
+let rec parent_hash_invariantP #bytes #cb #tkt #lp #ip t =
+  match t with
+  | TLeaf _ -> True
+  | TNode _ left right ->
+    node_has_parent_hash_linkP t /\
+    parent_hash_invariantP left /\
+    parent_hash_invariantP right
+
+(*** prop invariants lemmas ***)
+
+val node_has_parent_hash_linkP_intro: #bytes:Type0 -> {|crypto_bytes bytes|} -> #tkt:treekem_types bytes -> #lp:nat -> #lu:nat -> #ip:tree_index lp -> #iu:tree_index lu -> p:treesync bytes tkt lp ip{TNode? p /\ node_not_blank p} -> u:treesync bytes tkt lu iu ->
+  squash (lu < lp) ->
+  squash (leaf_index_inside lp ip iu) ->
+  squash (node_has_parent_hash u) ->
+  squash (is_subtree_of u p) ->
+  squash (last_update_correct u p) ->
+  squash (parent_hash_correct u p) ->
+  squash (node_has_parent_hash_linkP p)
+let node_has_parent_hash_linkP_intro #bytes #cb #tkt #lp #lu #ip #iu p u _ _ _ _ _ _ =
+  introduce exists (lu:nat) (iu:tree_index lu) (u:treesync bytes tkt lu iu). lu < lp /\ leaf_index_inside lp ip iu /\ node_has_parent_hash u /\ parent_hash_linkedP u p
+  with lu iu u
+  and ()
+
+
+val leaf_at_subtree: #bytes:Type0 -> {|crypto_bytes bytes|} -> #tkt:treekem_types bytes -> #lu:nat -> #lp:nat{lu <= lp} -> #iu:tree_index lu -> #ip:tree_index lp{leaf_index_inside lp ip iu} -> u:treesync bytes tkt lu iu -> p:treesync bytes tkt lp ip -> li:leaf_index lp ip -> Lemma
+  (requires leaf_index_inside lu iu li /\ is_subtree_of u p)
+  (ensures leaf_at p li == leaf_at u li)
+let rec leaf_at_subtree #bytes #cb #tkt #lu #lp #iu #ip u p li =
+  if lu = lp then ()
+  else (
+    leaf_index_same_side lu lp iu ip li;
+    let (p_child, _) = get_child_sibling p iu in
+    leaf_at_subtree u p_child li
+  )
+
+(*** is_subtree_of lemmas ***)
+
+#push-options "--fuel 2 --ifuel 1"
+val is_subtree_of_left_right: #bytes:Type0 -> {|bytes_like bytes|} -> #tkt:treekem_types bytes -> #lu:pos -> #lp:nat{lu <= lp} -> #iu:tree_index lu -> #ip:tree_index lp{leaf_index_inside lp ip iu} -> u:treesync bytes tkt lu iu -> p:treesync bytes tkt lp ip -> Lemma
+  (requires is_subtree_of u p)
+  (ensures (
+    match u with
+    | TNode _ left right -> is_subtree_of left p /\ is_subtree_of right p
+  ))
+let rec is_subtree_of_left_right #bytes #bl #tkt #lu #lp #iu #ip u p =
+  if lu = lp then (
+    ()
+  ) else (
+    let (p_child, _) = get_child_sibling p iu in
+    is_subtree_of_left_right u p_child
+  )
+#pop-options
+
+(*** bool invariant <==> prop invariant ***)
+
+val node_has_parent_hash_link_bool2prop: #bytes:Type0 -> {|crypto_bytes bytes|} -> #tkt:treekem_types bytes -> #lu:nat -> #lp:nat{lu < lp} -> #iu:tree_index lu -> #ip:tree_index lp{leaf_index_inside lp ip iu} -> u:treesync bytes tkt lu iu -> p:treesync bytes tkt lp ip{node_not_blank p} -> Lemma
+  (requires is_subtree_of u p /\ node_has_parent_hash_link_aux u p)
+  (ensures node_has_parent_hash_linkP p)
+let rec node_has_parent_hash_link_bool2prop #bytes #cb #tkt #lu #lp #iu #ip u p =
+  match u with
+  | TLeaf None -> ()
+  | TLeaf (Some lp) -> (
+    match lp.data.source with
+    | LNS_commit () -> ()
+    | _ -> ()
+  )
+  | TNode (Some kp) _ _ -> ()
+  | TNode None left right -> (
+    is_subtree_of_left_right u p;
+    if node_has_parent_hash_link_aux left p then (
+        node_has_parent_hash_link_bool2prop left p
+    ) else (
+        node_has_parent_hash_link_bool2prop right p
+    )
+  )
+
+val parent_hash_invariant_bool2prop: #bytes:Type0 -> {|crypto_bytes bytes|} -> #tkt:treekem_types bytes -> #l:nat -> #i:tree_index l -> t:treesync bytes tkt l i -> Lemma
+  (requires parent_hash_invariant t)
+  (ensures parent_hash_invariantP t)
+let rec parent_hash_invariant_bool2prop #bytes #cb #tkt #lp #ip t =
+  match t with
+  | TLeaf _ -> ()
+  | TNode opn left right -> (
+    parent_hash_invariant_bool2prop left;
+    parent_hash_invariant_bool2prop right;
+    match opn with
+    | None -> ()
+    | Some _ ->
+      is_subtree_of_left_right t t; //This lemma is needed, or a fuel of 2
+      if node_has_parent_hash_link_aux left t then (
+        node_has_parent_hash_link_bool2prop left t
+      ) else (
+        node_has_parent_hash_link_bool2prop right t
+      )
+  )
+
+#push-options "--z3rlimit 100"
+val node_has_parent_hash_link_aux_prop2bool:
+  #bytes:Type0 -> {|crypto_bytes bytes|} -> #tkt:treekem_types bytes ->
+  #lu:nat -> #lp:nat{lu < lp} -> #lt:nat{lu <= lt /\ lt < lp} -> #iu:tree_index lu -> #ip:tree_index lp{leaf_index_inside lp ip iu} -> #it:tree_index lt{leaf_index_inside lt it iu /\ leaf_index_inside lp ip it} ->
+  u:treesync bytes tkt lu iu{node_has_parent_hash u} -> p:treesync bytes tkt lp ip{node_not_blank p} -> t:treesync bytes tkt lt it ->
+  res_subset:(x:node_index{List.Tot.mem x (resolution t)} -> squash (let (p_child, _) = get_child_sibling p iu in List.Tot.mem x (resolution p_child))) ->
+  Lemma
+  (requires parent_hash_linkedP u p /\ u `is_subtree_of` t)
+  (ensures node_has_parent_hash_link_aux t p)
+let rec node_has_parent_hash_link_aux_prop2bool #bytes #cb #tkt #lu #lp #lt #iu #ip #it u p t res_subset =
+  if lu = lt then (
+    ()
+  ) else (
+    match t with
+    | TLeaf _ -> assert(False)
+    | TNode opn left right -> (
+      match opn with
+      | None -> (
+        let (t_child, t_sibling) = get_child_sibling t iu in
+        node_has_parent_hash_link_aux_prop2bool u p t_child (fun x -> List.Tot.append_mem (resolution left) (resolution right) x; res_subset x)
+      )
+      | Some _ -> (
+        res_subset (|lt, it|);
+        mem_last_update_lhs_eq u p (|lt, it|);
+        mem_last_update_rhs_eq u p (|lt, it|);
+        set_eq_to_set_eqP (last_update_lhs u p) (last_update_rhs u p);
+        assert(False)
+      )
+    )
+  )
+#pop-options
+
+#push-options "--z3rlimit 100"
+val parent_hash_invariant_prop2bool: #bytes:Type0 -> {|crypto_bytes bytes|} -> #tkt:treekem_types bytes -> #l:nat -> #i:tree_index l -> t:treesync bytes tkt l i -> Lemma
+  (requires parent_hash_invariantP t)
+  (ensures parent_hash_invariant t)
+let rec parent_hash_invariant_prop2bool #bytes #cb #tkt #l #i t =
+  match t with
+  | TLeaf _ -> ()
+  | TNode opn left right -> (
+    parent_hash_invariant_prop2bool left;
+    parent_hash_invariant_prop2bool right;
+    match opn with
+    | None -> ()
+    | Some _ -> (
+      eliminate exists (lu:nat) (iu:tree_index lu) (u:treesync bytes tkt lu iu). (lu < l /\ leaf_index_inside l i iu /\ node_has_parent_hash u /\ parent_hash_linkedP u t)
+      returns parent_hash_invariant t
+      with _. (
+        let (t_child, _) = get_child_sibling t iu in
+        node_has_parent_hash_link_aux_prop2bool u t t_child (fun _ -> ())
+      )
+    )
+  )
+#pop-options
+
+(*** Parent-hash invariant: easy cases ***)
+
+val parent_hash_invariant_mk_blank_tree: #bytes:Type0 -> {|crypto_bytes bytes|} -> #tkt:treekem_types bytes -> l:nat -> i:tree_index l -> Lemma (parent_hash_invariant (mk_blank_tree l i <: treesync bytes tkt l i))
+let rec parent_hash_invariant_mk_blank_tree #bytes #cb #tkt l i =
+  if l = 0 then ()
+  else (
+    parent_hash_invariant_mk_blank_tree #bytes #cb #tkt (l-1) (left_index i);
+    parent_hash_invariant_mk_blank_tree #bytes #cb #tkt (l-1) (right_index i)
+  )
+
+val parent_hash_invariant_add_one_level: #bytes:Type0 -> {|crypto_bytes bytes|} -> #tkt:treekem_types bytes -> #l:nat -> t:treesync bytes tkt l 0 -> Lemma
+  (requires parent_hash_invariant t)
+  (ensures parent_hash_invariant (add_one_level t))
+let extend_parent_hash_invariant #bytes #cb #tkt #l t =
+  parent_hash_invariant_mk_blank_tree #bytes #cb #tkt l (right_index #(l+1) 0)
+
+val parent_hash_invariant_canonicalize_tree: #bytes:Type0 -> {|crypto_bytes bytes|} -> #tkt:treekem_types bytes -> #l:nat -> t:treesync bytes tkt l 0 -> Lemma
+  (requires parent_hash_invariant t)
+  (ensures (let (|_, res_t|) = canonicalize_tree t in parent_hash_invariant res_t))
+let parent_hash_invariant_canonicalize_tree #l t = ()
+
+val parent_hash_invariant_tree_update: #bytes:Type0 -> {|crypto_bytes bytes|} -> #tkt:treekem_types bytes -> #l:nat -> #i:tree_index l -> t:treesync bytes tkt l i -> li:leaf_index l i -> ln:leaf_node_nt bytes tkt -> Lemma
+  (requires parent_hash_invariant t)
+  (ensures parent_hash_invariant (tree_update t li ln))
+let rec parent_hash_invariant_tree_update #bytes #cb #tkt #l #i t li ln =
+  match t with
+  | TLeaf _ -> ()
+  | TNode _ left right ->
+    if is_left_leaf li then
+      parent_hash_invariant_tree_update left li ln
+    else
+      parent_hash_invariant_tree_update right li ln
+
+val parent_hash_invariant_tree_remove: #bytes:Type0 -> {|crypto_bytes bytes|} -> #tkt:treekem_types bytes -> #l:nat -> #i:tree_index l -> t:treesync bytes tkt l i -> li:leaf_index l i -> Lemma
+  (requires parent_hash_invariant t)
+  (ensures parent_hash_invariant (tree_remove t li))
+let rec parent_hash_invariant_tree_remove #bytes #cb #tkt #l #i t li =
+  match t with
+  | TLeaf _ -> ()
+  | TNode _ left right ->
+    if is_left_leaf li then
+      parent_hash_invariant_tree_remove left li
+    else
+      parent_hash_invariant_tree_remove right li
+
+
+(*** Parent-hash invariant: adding inside ***)
+
+val add_inside_subtree: #bytes:Type0 -> {|bytes_like bytes|} -> #tkt:treekem_types bytes -> #lu:nat -> #lp:nat{lu <= lp} -> #iu:tree_index lu -> #ip:tree_index lp{leaf_index_inside lp ip iu} -> u:treesync bytes tkt lu iu -> p:treesync bytes tkt lp ip -> li:leaf_index lp ip{leaf_index_inside lu iu li} -> content:leaf_node_nt bytes tkt -> Lemma
+  (requires is_subtree_of u p /\ tree_add_pre u li /\ tree_add_pre p li)
+  (ensures is_subtree_of (tree_add u li content) (tree_add p li content))
+let rec add_inside_subtree #bytes #bl #tkt #lu #lp #iu #ip u p li content =
+  if lu = lp then ()
+  else (
+    let (p_child, _) = get_child_sibling p iu in
+    leaf_index_same_side lu lp iu ip li;
+    add_inside_subtree u p_child li content
+  )
+
+val mem_resolution_add_eq: #bytes:Type0 -> {|bytes_like bytes|} -> #tkt:treekem_types bytes -> #l:nat -> #i:tree_index l -> t:treesync bytes tkt l i -> li:leaf_index l i{leaf_at t li == None} -> content:leaf_node_nt bytes tkt -> x:node_index -> Lemma
+  (requires tree_add_pre t li)
+  (ensures List.Tot.mem x (resolution (tree_add t li content)) <==> (x == (|0, li|) \/ List.Tot.mem x (resolution t)))
+let rec mem_resolution_add_eq #bytes #bl #tkt #l #i t li content x =
+  let open MLS.TreeCommon in
+  match t with
+  | TLeaf None -> ()
+  | TNode None left right ->
+    if is_left_leaf li then (
+      mem_resolution_add_eq left li content x;
+      List.Tot.append_mem (resolution (tree_add left li content)) (resolution right) x;
+      List.Tot.append_mem (resolution left) (resolution right) x
+    ) else (
+      mem_resolution_add_eq right li content x;
+      List.Tot.append_mem (resolution left) (resolution (tree_add right li content)) x;
+      List.Tot.append_mem (resolution left) (resolution right) x
+    )
+  | TNode (Some c) _ _ -> (
+    let (|xl, xi|) = x in
+    FStar.Classical.forall_intro (mem_ul_insert_sorted li c.unmerged_leaves);
+    mem_unmerged_resolution_eq (insert_sorted li c.unmerged_leaves) x;
+    mem_unmerged_resolution_eq c.unmerged_leaves x
+  )
+
+
+#push-options "--z3rlimit 100"
+val add_inside_last_update: #bytes:Type0 -> {|bytes_like bytes|} -> #tkt:treekem_types bytes -> #lu:nat -> #lp:nat{lu < lp} -> #iu:tree_index lu -> #ip:tree_index lp{leaf_index_inside lp ip iu} -> u:treesync bytes tkt lu iu -> p:treesync bytes tkt lp ip{node_not_blank p} -> li:leaf_index lp ip{leaf_index_inside lu iu li /\ leaf_at p li == None /\ leaf_at u li == None} -> content:leaf_node_nt bytes tkt -> Lemma
+  (requires last_update_correct u p /\ tree_add_pre u li /\ tree_add_pre p li)
+  (ensures last_update_correct (tree_add u li content) (tree_add p li content))
+let add_inside_last_update #bytes #bl #tkt #lu #lp #iu #ip u p li content =
+  let (c, _) = get_child_sibling p iu in
+  let new_u = tree_add u li content in
+  let new_p = tree_add p li content in
+  let (new_c, _) = get_child_sibling new_p iu in
+  leaf_index_same_side lu lp iu ip li;
+  introduce forall x. List.Tot.mem x (last_update_lhs new_u new_p) <==> (List.Tot.mem x (last_update_lhs u p) \/ x == (|0, li|))
+  with (
+    mem_last_update_lhs_eq new_u new_p x;
+    mem_last_update_lhs_eq u p x;
+    mem_resolution_add_eq c li content x;
+    blank_leaf_not_in_resolution c li // Proves (|0, li|) != (|lu, iu|)
+  );
+  introduce forall x. List.Tot.mem x (last_update_rhs new_u new_p) <==> (List.Tot.mem x (last_update_rhs u p) \/ x == (|0, li|))
+  with (
+    mem_last_update_rhs_eq new_u new_p x;
+    mem_last_update_rhs_eq u p x;
+    let (|xl, xi|) = x in
+    let p_unmerged_leaves = (Some?.v (TNode?.data p)).unmerged_leaves in
+    mem_ul_insert_sorted li p_unmerged_leaves xi
+  );
+  set_eq_to_set_eqP (last_update_lhs u p) (last_update_rhs u p);
+  set_eqP_to_set_eq (last_update_lhs new_u new_p) (last_update_rhs new_u new_p);
+  mem_resolution_add_eq c li content (|lu, iu|)
+#pop-options
+
+val un_add_new_leaf_not_in_tree_lemma: #bytes:Type0 -> {|bytes_like bytes|} -> #tkt:treekem_types bytes -> #l:nat -> #i:tree_index l -> t:treesync bytes tkt l i -> unmerged_leaves: list (nat_lbytes 4) -> leaf:(nat_lbytes 4) -> leaves:list (nat_lbytes 4) -> Lemma
+  (requires List.Tot.for_all (unmerged_leaf_exists t) unmerged_leaves /\ (~(leaf_index_inside l i leaf)))
+  (ensures List.Tot.filter (un_add_unmerged_leaf (insert_sorted leaf leaves)) unmerged_leaves == List.Tot.filter (un_add_unmerged_leaf leaves) unmerged_leaves)
+let rec un_add_new_leaf_not_in_tree_lemma #bytes #bl #tkt #l #i t unmerged_leaves leaf leaves =
+  match unmerged_leaves with
+  | [] -> ()
+  | h_ul::t_ul ->
+    mem_ul_insert_sorted leaf leaves h_ul;
+    un_add_new_leaf_not_in_tree_lemma t t_ul leaf leaves
+
+val un_add_new_leaf_not_in_tree: #bytes:Type0 -> {|bytes_like bytes|} -> #tkt:treekem_types bytes -> #l:nat -> #i:tree_index l -> t:treesync bytes tkt l i -> leaves:list (nat_lbytes 4) -> leaf:nat_lbytes 4 -> Lemma
+  (requires ~(leaf_index_inside_tree t leaf))
+  (ensures un_add t leaves == un_add t (insert_sorted leaf leaves))
+let rec un_add_new_leaf_not_in_tree #bytes #bl #tkt #l #i t leaves leaf =
+  match t with
+  | TLeaf None -> ()
+  | TLeaf (Some _) -> mem_ul_insert_sorted leaf leaves i
+  | TNode opt_content left right -> (
+    un_add_new_leaf_not_in_tree left leaves leaf;
+    un_add_new_leaf_not_in_tree right leaves leaf;
+    match opt_content with
+    | None -> ()
+    | Some content -> (
+      un_add_new_leaf_not_in_tree_lemma t content.unmerged_leaves leaf leaves
+    )
+  )
+
+val add_inside_parent_hash: #bytes:Type0 -> {|crypto_bytes bytes|} -> #tkt:treekem_types bytes -> #lu:nat -> #lp:nat{lu < lp} -> #iu:tree_index lu -> #ip:tree_index lp{leaf_index_inside lp ip iu} -> u:treesync bytes tkt lu iu{node_has_parent_hash u} -> p:treesync bytes tkt lp ip{node_not_blank p} -> li:leaf_index lp ip{leaf_index_inside lu iu li /\ leaf_at p li == None /\ leaf_at u li == None} -> content:leaf_node_nt bytes tkt -> Lemma
+  (requires parent_hash_correct u p /\ tree_add_pre u li /\ tree_add_pre p li)
+  (ensures parent_hash_correct (tree_add u li content) (tree_add p li content))
+let add_inside_parent_hash #bytes #cb #tkt #lu #lp #iu #ip u p li content =
+  let p_content = (Some?.v (TNode?.data p)) in
+  let (p_child, p_sibling) = get_child_sibling p iu in
+  leaf_index_same_side lu lp iu ip li;
+  un_add_new_leaf_not_in_tree p_sibling p_content.unmerged_leaves li
+
+(*** Parent-hash invariant: adding outside ***)
+
+val add_outside_subtree: #bytes:Type0 -> {|bytes_like bytes|} -> #tkt:treekem_types bytes -> #lu:nat -> #lp:nat{lu <= lp} -> #iu:tree_index lu -> #ip:tree_index lp{leaf_index_inside lp ip iu} -> u:treesync bytes tkt lu iu -> p:treesync bytes tkt lp ip -> li:leaf_index lp ip{~(leaf_index_inside lu iu li) /\ leaf_at p li == None} -> content:leaf_node_nt bytes tkt -> Lemma
+  (requires is_subtree_of u p /\ tree_add_pre p li)
+  (ensures is_subtree_of u (tree_add p li content))
+let rec add_outside_subtree #bytes #bl #tkt #lu #lp #iu #ip u p li content =
+  if lu = lp then ()
+  else (
+    let (p_child, _) = get_child_sibling p iu in
+    if leaf_index_inside_tree p_child li then (
+      add_outside_subtree u p_child li content
+    ) else ()
+  )
+
+val add_outside_last_update_aux: pred:(nat_lbytes 4 -> bool) -> li:nat_lbytes 4 -> p_unmerged_leaves:list (nat_lbytes 4) -> Lemma
+  (requires ~(pred li))
+  (ensures List.Tot.filter pred p_unmerged_leaves == List.Tot.filter pred (insert_sorted li p_unmerged_leaves))
+let rec add_outside_last_update_aux pred li p_unmerged_leaves =
+  match p_unmerged_leaves with
+  | [] -> ()
+  | h::t ->
+    if li < h then ()
+    else if li = h then ()
+    else add_outside_last_update_aux pred li t
+
+#push-options "--z3rlimit 100"
+val add_outside_last_update: #bytes:Type0 -> {|bytes_like bytes|} -> #tkt:treekem_types bytes -> #lu:nat -> #lp:nat{lu < lp} -> #iu:tree_index lu -> #ip:tree_index lp{leaf_index_inside lp ip iu} -> u:treesync bytes tkt lu iu -> p:treesync bytes tkt lp ip{node_not_blank p} -> li:leaf_index lp ip{~(leaf_index_inside lu iu li) /\ leaf_at p li == None} -> content:leaf_node_nt bytes tkt -> Lemma
+  (requires last_update_correct u p /\ tree_add_pre p li)
+  (ensures last_update_correct u (tree_add p li content))
+let add_outside_last_update #bytes #bl #tkt #lu #lp #iu #ip u p li content =
+  let (c, _) = get_child_sibling p iu in
+  let new_p = tree_add p li content in
+  if leaf_index_inside_tree c li then (
+    introduce forall x. List.Tot.mem x (last_update_lhs u new_p) <==> (List.Tot.mem x (last_update_lhs u p) \/ x == (|0, li|))
+    with (
+      mem_last_update_lhs_eq u new_p x;
+      mem_last_update_lhs_eq u p x;
+      mem_resolution_add_eq c li content x;
+      blank_leaf_not_in_resolution c li // Proves (|0, li|) != (|lu, iu|)
+    );
+    introduce forall x. List.Tot.mem x (last_update_rhs u new_p) <==> (List.Tot.mem x (last_update_rhs u p) \/ x == (|0, li|))
+    with (
+      mem_last_update_rhs_eq u new_p x;
+      mem_last_update_rhs_eq u p x;
+      let p_unmerged_leaves = (Some?.v (TNode?.data p)).unmerged_leaves in
+      let (|xl, xi|) = x in
+      mem_ul_insert_sorted li p_unmerged_leaves xi
+    );
+    set_eq_to_set_eqP (last_update_lhs u p) (last_update_rhs u p);
+    set_eqP_to_set_eq (last_update_lhs u new_p) (last_update_rhs u new_p);
+    mem_resolution_add_eq c li content (|lu, iu|)
+  ) else (
+    let p_unmerged_leaves = (Some?.v (TNode?.data p)).unmerged_leaves in
+    add_outside_last_update_aux (leaf_index_inside_tree c) li p_unmerged_leaves
+  )
+#pop-options
+
+val un_add_add_lemma_lemma: #bytes:Type0 -> {|bytes_like bytes|} -> #tkt:treekem_types bytes -> #l:nat -> #i:tree_index l -> t:treesync bytes tkt l i -> li:leaf_index l i -> unmerged_leaves:list (nat_lbytes 4) -> leaves:list (nat_lbytes 4) -> Lemma
+  (requires (~(unmerged_leaf_exists t li)) /\ (List.Tot.for_all (unmerged_leaf_exists t) unmerged_leaves) /\ li < pow2 32)
+  (ensures List.Tot.filter (un_add_unmerged_leaf leaves) unmerged_leaves == List.Tot.filter (un_add_unmerged_leaf (insert_sorted li leaves)) unmerged_leaves)
+let rec un_add_add_lemma_lemma #bytes #bl #tkt #l #i t li unmerged_leaves leaves =
+  match unmerged_leaves with
+  | [] -> ()
+  | head_ul::tail_ul ->
+    mem_ul_insert_sorted li leaves head_ul;
+    un_add_add_lemma_lemma t li tail_ul leaves
+
+#push-options "--fuel 2 --ifuel 1"
+val un_add_add_lemma: #bytes:Type0 -> {|bytes_like bytes|} -> #tkt:treekem_types bytes -> #l:nat -> #i:tree_index l -> t:treesync bytes tkt l i -> li:leaf_index l i -> unmerged_leaves:list (nat_lbytes 4) -> leaves:list (nat_lbytes 4) -> Lemma
+  (requires (~(unmerged_leaf_exists t li)) /\ (List.Tot.for_all (unmerged_leaf_exists t) unmerged_leaves) /\ li < pow2 32)
+  (ensures List.Tot.filter (un_add_unmerged_leaf leaves) unmerged_leaves == List.Tot.filter (un_add_unmerged_leaf (insert_sorted li leaves)) (insert_sorted li unmerged_leaves))
+let rec un_add_add_lemma #bytes #bl #tkt #l #i t li unmerged_leaves leaves =
+  match unmerged_leaves with
+  | [] -> (
+    mem_ul_insert_sorted li leaves li
+  )
+  | head_ul::tail_ul -> (
+    if li < head_ul then (
+      mem_ul_insert_sorted li leaves li;
+      un_add_add_lemma_lemma t li unmerged_leaves leaves
+    )
+    else if li = head_ul then ()
+    else (
+      mem_ul_insert_sorted li leaves head_ul;
+      un_add_add_lemma t li tail_ul leaves
+    )
+  )
+#pop-options
+
+val un_add_add: #bytes:Type0 -> {|bytes_like bytes|} -> #tkt:treekem_types bytes -> #l:nat -> #i:tree_index l -> t:treesync bytes tkt l i -> li:leaf_index l i{leaf_at t li == None} -> content:leaf_node_nt bytes tkt -> leaves:list (nat_lbytes 4) -> Lemma
+  (requires tree_add_pre t li /\ li < pow2 32)
+  (ensures un_add (tree_add t li content) (insert_sorted li leaves) == un_add t leaves)
+let rec un_add_add #bytes #bl #tkt #l #i t li content leaves =
+  match t with
+  | TLeaf _ -> mem_ul_insert_sorted li leaves li
+  | TNode opt_cont left right ->
+    (if is_left_leaf li then (
+      un_add_add left li content leaves;
+      un_add_new_leaf_not_in_tree right leaves li
+    ) else (
+      un_add_add right li content leaves;
+      un_add_new_leaf_not_in_tree left leaves li
+    ));
+    match opt_cont with
+    | None -> ()
+    | Some cont -> (
+      un_add_add_lemma t li cont.unmerged_leaves leaves
+    )
+
+#push-options "--z3rlimit 100"
+val add_outside_parent_hash: #bytes:Type0 -> {|crypto_bytes bytes|} -> #tkt:treekem_types bytes -> #lu:nat -> #lp:nat{lu < lp} -> #iu:tree_index lu -> #ip:tree_index lp{leaf_index_inside lp ip iu} -> u:treesync bytes tkt lu iu{node_has_parent_hash u} -> p:treesync bytes tkt lp ip{node_not_blank p} -> li:leaf_index lp ip{~(leaf_index_inside lu iu li) /\ leaf_at p li == None} -> content:leaf_node_nt bytes tkt -> Lemma
+  (requires parent_hash_correct u p /\ tree_add_pre p li)
+  (ensures parent_hash_correct u (tree_add p li content))
+let add_outside_parent_hash #bytes #cb #tkt #lu #lp #iu #ip u p li content =
+  let new_p = tree_add p li content in
+  let p_content = (Some?.v (TNode?.data p)) in
+  let new_p_content = (Some?.v (TNode?.data new_p)) in
+  let (c, s) = get_child_sibling p iu in
+  let (new_c, new_s) = get_child_sibling new_p iu in
+  if leaf_index_inside_tree c li then (
+    assert(~(leaf_index_inside_tree s li));
+    assert(li < pow2 32);
+    un_add_new_leaf_not_in_tree s p_content.unmerged_leaves li
+  ) else (
+    un_add_add s li content p_content.unmerged_leaves
+  )
+#pop-options
+
+val tree_add_pre_subtree_inside: #bytes:Type0 -> {|bytes_like bytes|} -> #tkt:treekem_types bytes -> #lu:nat -> #lp:nat{lu <= lp} -> #iu:tree_index lu -> #ip:tree_index lp{leaf_index_inside lp ip iu} -> u:treesync bytes tkt lu iu -> p:treesync bytes tkt lp ip -> li:leaf_index lp ip{leaf_index_inside lu iu li} -> content:leaf_node_nt bytes tkt -> Lemma
+  (requires is_subtree_of u p /\ tree_add_pre p li)
+  (ensures tree_add_pre u li)
+let rec tree_add_pre_subtree_inside #bytes #bl #tkt #lu #lp #iu #ip u p li content =
+  if lu = lp then ()
+  else (
+    leaf_index_same_side lu lp iu ip li;
+    let (child, sibling) = get_child_sibling p iu in
+    tree_add_pre_subtree_inside u child li content
+  )
+
+(*** Parent-hash invariant: tree add final proof ***)
+
+#push-options "--z3rlimit 100"
+val parent_hash_invariantP_tree_add: #bytes:Type0 -> {|crypto_bytes bytes|} -> #tkt:treekem_types bytes -> #l:nat -> #i:tree_index l -> t:treesync bytes tkt l i -> li:leaf_index l i{leaf_at t li == None} -> content:leaf_node_nt bytes tkt -> Lemma
+  (requires parent_hash_invariantP t /\ tree_add_pre t li)
+  (ensures parent_hash_invariantP (tree_add t li content))
+let rec parent_hash_invariantP_tree_add #bytes #cb #tkt #l #i t li content =
+  match t with
+  | TLeaf content -> ()
+  | TNode opt_content left right ->
+    (
+    if is_left_leaf li then
+      parent_hash_invariantP_tree_add left li content
+    else
+      parent_hash_invariantP_tree_add right li content
+    );
+    match opt_content with
+    | None -> ()
+    | Some node_content -> (
+      eliminate exists (lu:nat) (iu:tree_index lu) (u:treesync bytes tkt lu iu). (lu < l /\ leaf_index_inside l i iu /\ node_has_parent_hash u /\ parent_hash_linkedP u t)
+      returns (node_has_parent_hash_linkP (tree_add t li content))
+      with _. (
+        if leaf_index_inside lu iu li then (
+          tree_add_pre_subtree_inside u t li content;
+          leaf_at_subtree u t li;
+          node_has_parent_hash_linkP_intro (tree_add t li content) (tree_add u li content) () () () (
+            add_inside_subtree u t li content
+          ) (
+            add_inside_last_update u t li content
+          ) (
+            add_inside_parent_hash u t li content
+          )
+        ) else (
+          node_has_parent_hash_linkP_intro (tree_add t li content) u () () () (
+            add_outside_subtree u t li content
+          ) (
+            add_outside_last_update u t li content
+          ) (
+            add_outside_parent_hash u t li content
+          )
+        )
+      )
+    )
+#pop-options
+
+val parent_hash_invariant_tree_add: #bytes:Type0 -> {|crypto_bytes bytes|} -> #tkt:treekem_types bytes -> #l:nat -> #i:tree_index l -> t:treesync bytes tkt l i -> li:leaf_index l i{leaf_at t li == None} -> content:leaf_node_nt bytes tkt -> Lemma
+  (requires parent_hash_invariant t /\ tree_add_pre t li)
+  (ensures parent_hash_invariant (tree_add t li content))
+let parent_hash_invariant_tree_add #bytes #cb #tkt #l #i t li content =
+  parent_hash_invariant_bool2prop t;
+  parent_hash_invariantP_tree_add t li content;
+  parent_hash_invariant_prop2bool (tree_add t li content)
+
+(*** Parent-hash invariant: applying external path ***)
+
+val find_parent_hash_link_aux: #bytes:Type0 -> {|crypto_bytes bytes|} -> #tkt:treekem_types bytes -> #l:nat -> #i:tree_index l -> #li:leaf_index l i -> t:treesync bytes tkt l i -> p:external_pathsync bytes tkt l i li -> parent_parent_hash:mls_bytes bytes -> Pure (lu:nat & iu:tree_index lu & treesync bytes tkt lu iu)
+  (requires apply_external_path_aux_pre t p (length #bytes parent_parent_hash))
+  (ensures fun _ -> True)
+let rec find_parent_hash_link_aux #bytes #cb #tkt #l #i #li t p parent_parent_hash =
+  match t, p with
+  | TLeaf _, PLeaf _ ->
+    (|l, i, apply_external_path_aux t p parent_parent_hash|)
+  | TNode _ _ _, PNode (Some _) _ -> (
+    (|l, i, apply_external_path_aux t p parent_parent_hash|)
+  )
+  | TNode _ left right, PNode None p_next -> (
+    if is_left_leaf li then
+      find_parent_hash_link_aux left p_next parent_parent_hash
+    else
+      find_parent_hash_link_aux right p_next parent_parent_hash
+  )
+
+val path_node_not_blank: #bytes:Type0 -> {|crypto_bytes bytes|} -> #tkt:treekem_types bytes -> #l:nat -> #i:tree_index l -> #li:leaf_index l i -> external_pathsync bytes tkt l i li -> bool
+let path_node_not_blank #bytes #cb #tkt #l #i #li p =
+  match p with
+  | PLeaf _ -> true
+  | PNode (Some _) _ -> true
+  | _ -> false
+
+val find_parent_hash_link: #bytes:Type0 -> {|crypto_bytes bytes|} -> #tkt:treekem_types bytes -> #l:pos -> #i:tree_index l -> #li:leaf_index l i -> t:treesync bytes tkt l i -> p:external_pathsync bytes tkt l i li{path_node_not_blank p} -> parent_parent_hash:mls_bytes bytes -> Pure (lu:nat & iu:tree_index lu & treesync bytes tkt lu iu)
+  (requires apply_external_path_aux_pre t p (length #bytes parent_parent_hash))
+  (ensures fun _ -> True)
+let find_parent_hash_link #bytes #cb #tkt #l #i #li t p parent_parent_hash =
+  match t, p with
+  | TNode _ left right, PNode opt_ext_content p_next -> (
+    let (child, sibling) = get_child_sibling t li in
+    let (_, new_parent_parent_hash) = compute_new_np_and_ph opt_ext_content sibling parent_parent_hash in
+    if is_left_leaf li then
+      find_parent_hash_link_aux left p_next new_parent_parent_hash
+    else
+      find_parent_hash_link_aux right p_next new_parent_parent_hash
+  )
+
+val external_path_is_parent_hash_valid_aux: #bytes:Type0 -> {|crypto_bytes bytes|} -> #tkt:treekem_types bytes -> #l:nat -> #i:tree_index l -> #li:leaf_index l i -> treesync bytes tkt l i -> external_pathsync bytes tkt l i li -> mls_bytes bytes -> bool
+let external_path_is_parent_hash_valid_aux #bytes #cb #tkt #l #i #li t p parent_parent_hash =
+  let new_lp = get_external_path_leaf p in
+  compute_leaf_parent_hash_from_external_path_pre t p (length #bytes parent_parent_hash) && (
+  let computed_parent_hash = compute_leaf_parent_hash_from_external_path t p parent_parent_hash in
+  (new_lp.data.source = LNS_commit () && (new_lp.data.parent_hash <: bytes) = computed_parent_hash)
+  )
+
+val is_tree_empty_implies_empty_resolution: #bytes:Type0 -> {|bytes_like bytes|} -> #tkt:treekem_types bytes -> #l:nat -> #i:tree_index l -> t:treesync bytes tkt l i -> Lemma
+  (requires is_tree_empty t)
+  (ensures resolution t == [])
+let rec is_tree_empty_implies_empty_resolution #bytes #bl #tkt #l #i t =
+  match t with
+  | TLeaf None -> ()
+  | TNode None left right -> (
+    is_tree_empty_implies_empty_resolution left;
+    is_tree_empty_implies_empty_resolution right
+  )
+
+#push-options "--z3rlimit 100"
+//Properties that are just (almost) trivial induction
+val find_parent_hash_link_aux_misc_properties: #bytes:Type0 -> {|crypto_bytes bytes|} -> #tkt:treekem_types bytes -> #l:nat -> #i:tree_index l -> #li:leaf_index l i -> t:treesync bytes tkt l i -> p:external_pathsync bytes tkt l i li -> parent_parent_hash:mls_bytes bytes -> Lemma
+  (requires external_path_is_parent_hash_valid_aux t p parent_parent_hash /\ external_path_is_filter_valid t p /\ apply_external_path_aux_pre t p (length #bytes parent_parent_hash))
+  (ensures (
+    let (|lu, iu, u|) = find_parent_hash_link_aux t p parent_parent_hash in
+    lu <= l /\
+    leaf_index_inside l i iu /\
+    node_has_parent_hash u /\
+    is_subtree_of u (apply_external_path_aux t p parent_parent_hash) /\
+    get_parent_hash_of u == parent_parent_hash /\
+    resolution (apply_external_path_aux t p parent_parent_hash) == [(|lu, iu|)] /\
+    True
+  ))
+let rec find_parent_hash_link_aux_misc_properties #bytes #cb #tkt #l #i #li t p parent_parent_hash =
+  match t, p with
+  | TLeaf _, PLeaf _ -> ()
+  | TNode _ _ _, PNode (Some _) _ -> ()
+  | TNode _ left right, PNode None p_next ->
+    let (child, sibling) = get_child_sibling t li in
+    let (new_opt_content, new_parent_parent_hash) = compute_new_np_and_ph None sibling parent_parent_hash in
+    let (|lu, iu, u|) = find_parent_hash_link_aux t p parent_parent_hash in
+    is_tree_empty_implies_empty_resolution sibling;
+    FStar.List.Tot.Properties.append_l_nil [(|lu, iu|)];
+    if is_left_leaf li then
+      find_parent_hash_link_aux_misc_properties left p_next new_parent_parent_hash
+    else
+      find_parent_hash_link_aux_misc_properties right p_next new_parent_parent_hash
+#pop-options
+
+#push-options "--z3rlimit 100"
+val find_parent_hash_link_misc_properties: #bytes:Type0 -> {|crypto_bytes bytes|} -> #tkt:treekem_types bytes -> #l:pos -> #i:tree_index l -> #li:leaf_index l i -> t:treesync bytes tkt l i -> p:external_pathsync bytes tkt l i li{path_node_not_blank p} -> parent_parent_hash:mls_bytes bytes -> Lemma
+  (requires external_path_is_parent_hash_valid_aux t p parent_parent_hash /\ external_path_is_filter_valid t p /\ apply_external_path_aux_pre t p (length #bytes parent_parent_hash))
+  (ensures (
+    let (|lu, iu, u|) = find_parent_hash_link t p parent_parent_hash in
+    lu < l /\
+    leaf_index_inside l i iu /\
+    node_has_parent_hash u /\
+    is_subtree_of u (apply_external_path_aux t p parent_parent_hash)
+  ))
+let find_parent_hash_link_misc_properties #bytes #cb #tkt #l #i #li t p parent_parent_hash =
+  match t, p with
+  | TNode _ left right, PNode opt_ext_content p_next -> (
+    let (child, sibling) = get_child_sibling t li in
+    let (_, new_parent_parent_hash) = compute_new_np_and_ph opt_ext_content sibling parent_parent_hash in
+    if is_left_leaf li then
+      find_parent_hash_link_aux_misc_properties left p_next new_parent_parent_hash
+    else
+      find_parent_hash_link_aux_misc_properties right p_next new_parent_parent_hash
+  )
+#pop-options
+
+#push-options "--fuel 2 --z3rlimit 100"
+val find_parent_hash_link_last_update: #bytes:Type0 -> {|crypto_bytes bytes|} -> #tkt:treekem_types bytes -> #l:pos -> #i:tree_index l -> #li:leaf_index l i -> t:treesync bytes tkt l i -> p:external_pathsync bytes tkt l i li{path_node_not_blank p} -> parent_parent_hash:mls_bytes bytes -> Lemma
+  (requires external_path_is_parent_hash_valid_aux t p parent_parent_hash /\ external_path_is_filter_valid t p /\ apply_external_path_aux_pre t p (length #bytes parent_parent_hash))
+  (ensures (
+    find_parent_hash_link_misc_properties t p parent_parent_hash;
+    let (|lu, iu, u|) = find_parent_hash_link t p parent_parent_hash in
+    last_update_correct u (apply_external_path_aux t p parent_parent_hash)
+  ))
+let find_parent_hash_link_last_update #bytes #cb #tkt #l #i #li t p parent_parent_hash =
+  find_parent_hash_link_misc_properties t p parent_parent_hash;
+  let (|lu, iu, u|) = find_parent_hash_link t p parent_parent_hash in
+  match t, p with
+  | TNode _ left right, PNode opt_ext_content p_next -> (
+    let (child, sibling) = get_child_sibling t li in
+    let (_, new_parent_parent_hash) = compute_new_np_and_ph opt_ext_content sibling parent_parent_hash in
+    find_parent_hash_link_aux_misc_properties child p_next new_parent_parent_hash;
+    if is_left_leaf li then (
+      find_parent_hash_link_aux_misc_properties left p_next new_parent_parent_hash
+    )
+    else
+      find_parent_hash_link_aux_misc_properties right p_next new_parent_parent_hash
+  )
+#pop-options
+
+val un_add_empty_lemma: l:list (nat_lbytes 4) -> Lemma (List.Tot.filter (un_add_unmerged_leaf []) l == l)
+let rec un_add_empty_lemma l =
+  match l with
+  | [] -> ()
+  | h::t -> un_add_empty_lemma t
+
+val un_add_empty: #bytes:Type0 -> {|bytes_like bytes|} -> #tkt:treekem_types bytes -> #l:nat -> #i:tree_index l -> t:treesync bytes tkt l i -> Lemma
+  (un_add t [] == t)
+let rec un_add_empty #bytes #tkt #l #i t =
+  match t with
+  | TLeaf _ -> ()
+  | TNode opt_content left right ->
+    un_add_empty left;
+    un_add_empty right;
+    match opt_content with
+    | None -> ()
+    | Some content -> un_add_empty_lemma content.unmerged_leaves
+
+val find_parent_hash_link_parent_hash: #bytes:Type0 -> {|crypto_bytes bytes|} -> #tkt:treekem_types bytes -> #l:pos -> #i:tree_index l -> #li:leaf_index l i -> t:treesync bytes tkt l i -> p:external_pathsync bytes tkt l i li{path_node_not_blank p} -> parent_parent_hash:mls_bytes bytes -> Lemma
+  (requires external_path_is_parent_hash_valid_aux t p parent_parent_hash /\ external_path_is_filter_valid t p /\ apply_external_path_aux_pre t p (length #bytes parent_parent_hash))
+  (ensures (
+    find_parent_hash_link_misc_properties t p parent_parent_hash;
+    let (|lu, iu, u|) = find_parent_hash_link t p parent_parent_hash in
+    parent_hash_correct u (apply_external_path_aux t p parent_parent_hash)
+  ))
+let find_parent_hash_link_parent_hash #bytes #cb #tkt #l #i #li t p parent_parent_hash =
+  match t, p with
+  | TNode _ left right, PNode (Some ext_content) p_next -> (
+    let (child, sibling) = get_child_sibling t li in
+    let (_, new_parent_parent_hash) = compute_new_np_and_ph (Some ext_content) sibling parent_parent_hash in
+    un_add_empty sibling;
+    if is_left_leaf li then (
+      find_parent_hash_link_aux_misc_properties left p_next new_parent_parent_hash
+    ) else
+      find_parent_hash_link_aux_misc_properties right p_next new_parent_parent_hash
+  )
+
+#push-options "--z3rlimit 100"
+val parent_hash_invariantP_apply_external_path_aux: #bytes:Type0 -> {|crypto_bytes bytes|} -> #tkt:treekem_types bytes -> #l:nat -> #i:tree_index l -> #li:leaf_index l i -> t:treesync bytes tkt l i -> p:external_pathsync bytes tkt l i li -> parent_parent_hash:mls_bytes bytes -> Lemma
+  (requires parent_hash_invariantP t /\ external_path_is_parent_hash_valid_aux t p parent_parent_hash /\ external_path_is_filter_valid t p /\ apply_external_path_aux_pre t p (length #bytes parent_parent_hash))
+  (ensures parent_hash_invariantP (apply_external_path_aux t p parent_parent_hash))
+let rec parent_hash_invariantP_apply_external_path_aux #bytes #cb #tkt #l #i #li t p parent_parent_hash =
+  match t, p with
+  | TLeaf content, PLeaf _ -> ()
+  | TNode opt_content left right, PNode opt_ext_content p_next ->
+    let (child, sibling) = get_child_sibling t li in
+    let (_, new_parent_parent_hash) = compute_new_np_and_ph opt_ext_content sibling parent_parent_hash in
+    (if is_left_leaf li then parent_hash_invariantP_apply_external_path_aux left p_next new_parent_parent_hash
+    else parent_hash_invariantP_apply_external_path_aux right p_next new_parent_parent_hash);
+    match opt_ext_content with
+    | None -> ()
+    | Some _ -> (
+      find_parent_hash_link_misc_properties t p parent_parent_hash;
+      let (|lu, iu, u|) = find_parent_hash_link t p parent_parent_hash in
+      node_has_parent_hash_linkP_intro (apply_external_path_aux t p parent_parent_hash) u () () () () (
+        find_parent_hash_link_last_update t p parent_parent_hash
+      ) (
+        find_parent_hash_link_parent_hash t p parent_parent_hash
+      )
+    )
+#pop-options
+
+val parent_hash_invariant_apply_external_path: #bytes:Type0 -> {|crypto_bytes bytes|} -> #tkt:treekem_types bytes -> #l:nat -> #li:leaf_index l 0 -> t:treesync bytes tkt l 0 -> p:external_pathsync bytes tkt l 0 li -> Lemma
+  (requires parent_hash_invariant t /\ external_path_is_parent_hash_valid t p /\ external_path_is_filter_valid t p /\ apply_external_path_pre t p)
+  (ensures parent_hash_invariant (apply_external_path t p))
+let parent_hash_invariant_apply_external_path #bytes #cb #tkt #l #li t p =
+  parent_hash_invariant_bool2prop t;
+  parent_hash_invariantP_apply_external_path_aux t p (root_parent_hash #bytes);
+  parent_hash_invariant_prop2bool (apply_external_path t p)
